<section xml:id="sec_implicit_functions">
  <title>Implicit Functions</title>
  <p>
    An implicit function defines a relationship between two (or more) variables differently from an explicit function.
    As opposed to an explicit function that can be written in the form of
    <me>
      y = f(x)
    </me>,
    an implicit function is defined as an <em>equation</em> of multiple variables. It is often the case that this equation cannot be solved for 
    one variable explicitly in terms of the other. In Maple, it is easiest to assign a name to the entire equation, including the <m>=</m> sign.
  </p>
  <p>
    The elliptic curve <m>y^2 = x^3 - 2*x + 1</m> is a simple example. It cannot be written as a single function of the form <m>y = f(x)</m>, 
    since for a given value of <m>x</m>, there may be two different <m>y</m>-values.
  </p>
  <console prompt="> ">
    <input>E := y^2 = x^3 - 2*x + 1;</input>
  </console>
  <p>
    <me>
      \displaystyle E\, := \,{y}^{2}={x}^{3}-2\,x+1
    </me>
  </p>
  <p>
    To find points on the curve, we can substitute a value for <m>x</m> and solve for <m>y</m>.
  </p>
  <console prompt="> ">
    <input>subs(x=2, E); solve(%,x);</input>
  </console>
  <p>
    <idx><h>subs</h></idx>
    <idx><h>solving equations</h><h>solve</h></idx>
    <idx><h>ditto operator</h></idx>
    <me>
      \displaystyle {y}^{2}=5
    </me>
    <me>
      \displaystyle  \sqrt{5},\,- \sqrt{5}
    </me>
  </p>
  <p>
    Although many implicit functions cannot be expressed as a single function <m>y=f(x)</m>, it may be possible to split up implicit functions into explicit functions by solving for <m>y</m>.
  </p>
  <console prompt="> ">
    <input>L := x^2 + (y - surd(x^2,3))^2 = 1;</input>
  </console>
  <aside>
    <p>
      Here, the command <c>surd(x^2,3)</c> is equivalent to <m>\sqrt[3]{x^2}</m>.
      You may also use <c>root[3](x^2)</c>, although the results may vary. Maple is built to work with complex numbers, which lead to some unusual behaviours with roots and exponents.
    </p>
  </aside>
  <p>
    <idx><h>mathematical functions</h><h><m>n</m>th root</h></idx>
    <me>
      \displaystyle L\, := \,{x}^{2}+ \left( y-\sqrt [3]{{x}^{2}} \right) ^{2}=1
    </me>
  </p>
  <console prompt="> ">
    <input>solve(L, y);</input>
  </console>
  <p>
    <me>
      \displaystyle \sqrt [3]{{x}^{2}}+ \sqrt{-{x}^{2}+1},\,\sqrt [3]{{x}^{2}}- \sqrt{-{x}^{2}+1}
    </me>
  </p>
</section>